Fetch macros

theories/examples/macros/fetch.v
@@ -1,14 +1,10 @@
-From iris.algebra Require Import frac.
 From iris.proofmode Require Import proofmode.
-From cap_machine.proofmode Require Import tactics_helpers map_simpl solve_pure.
-From cap_machine Require Import logrel addr_reg_sample fundamental rules proofmode.
-From cap_machine Require Export iris_extra addr_reg_sample contiguous.
+From cap_machine Require Import rules proofmode.
 
 Section Fetch.
   Context
     {Σ : gFunctors}
       {ceriseg: ceriseG Σ}
-      {nainv: logrel_na_invs Σ}
       {MP: MachineParameters}
   .
 
@@ -16,139 +12,60 @@ Section Fetch.
   (* ------------------------------------- FETCH ------------------------------------- *)
   (* --------------------------------------------------------------------------------- *)
 
-  Definition fetch_instrs (f : Z) :=
-    [move_r r_t1 PC;
-    getb r_t2 r_t1;
-    geta r_t3 r_t1;
-    sub_r_r r_t2 r_t2 r_t3;
-    lea_r r_t1 r_t2;
-    load_r r_t1 r_t1;
-    lea_z r_t1 f;
-    move_z r_t2 0;
-    move_z r_t3 0;
-    load_r r_t1 r_t1].
+  (** Fetch the value at the address (pc_b + n).
+     - rdst contains the fetched value.
+     - rscratch1 and rscratch2 are both clobbered.
+   **)
+  Definition fetch_instrs (n : Z) (rdst rscratch1 rscratch2 : RegName) : list Word :=
+    encodeInstrsW [
+      Mov rdst PC;
+      GetB rscratch1 rdst;
+      GetA rscratch2 rdst;
+      Sub rscratch1 rscratch1 rscratch2;
+      Lea rdst rscratch1;
+      Lea rdst n;
+      Load rdst rdst;
+      Mov rscratch1 0%Z;
+      Mov rscratch2 0%Z
+    ].
 
-  Definition fetch f a : iProp Σ :=
-    ([∗ list] a_i;w_i ∈ a;(fetch_instrs f), a_i ↦ₐ w_i)%I.
+  Lemma fetch_spec
+    (n : Z) (rdst rscratch1 rscratch2 : RegName) (la : list Addr)
+    (pc_p : Perm) (pc_g : Locality) (pc_b pc_e pc_a : Addr)
+    (wentry wdst w1 w2 : Word)
+    (φ : language.val cap_lang → iPropI Σ) :
 
-  (* fetch spec *)
-  Lemma fetch_spec f a pc_p pc_b pc_e a_first a_last b_link e_link a_link entry_a wentry φ w1 w2 w3:
-    isCorrectPC_range pc_p pc_b pc_e a_first a_last ->
-    contiguous_between a a_first a_last ->
-    withinBounds b_link e_link entry_a = true ->
-    (a_link + f)%a = Some entry_a ->
+    let fetch := (fetch_instrs n rdst rscratch1 rscratch2) in
+    let a_last := (pc_a ^+ length fetch)%a in
+    executeAllowed pc_p = true →
+    SubBounds pc_b pc_e pc_a a_last →
+    withinBounds pc_b pc_e (pc_b ^+ n)%a = true ->
 
-      ▷ fetch f a
-    ∗ ▷ PC ↦ᵣ WCap pc_p pc_b pc_e a_first
-    ∗ ▷ pc_b ↦ₐ WCap RO b_link e_link a_link
-    ∗ ▷ entry_a ↦ₐ wentry
-    ∗ ▷ r_t1 ↦ᵣ w1
-    ∗ ▷ r_t2 ↦ᵣ w2
-    ∗ ▷ r_t3 ↦ᵣ w3
-    (* if the capability is global, we want to be able to continue *)
-    (* if w is not a global capability, we will fail, and must now show that Phi holds at failV *)
-    ∗ ▷ (PC ↦ᵣ WCap pc_p pc_b pc_e a_last ∗ fetch f a
-            (* the newly allocated region *)
-            ∗ r_t1 ↦ᵣ wentry ∗ r_t2 ↦ᵣ WInt 0%Z ∗ r_t3 ↦ᵣ WInt 0%Z
-            ∗ pc_b ↦ₐ WCap RO b_link e_link a_link
-            ∗ entry_a ↦ₐ wentry
-            -∗ WP Seq (Instr Executable) {{ φ }})
-    ⊢
-      WP Seq (Instr Executable) {{ φ }}.
+    ▷ PC ↦ᵣ WCap pc_p pc_g pc_b pc_e pc_a
+    ∗ ▷ rdst ↦ᵣ wdst
+    ∗ ▷ rscratch1 ↦ᵣ w1
+    ∗ ▷ rscratch2 ↦ᵣ w2
+    ∗ ▷ codefrag pc_a fetch
+    ∗ ▷ (pc_b ^+ n)%a ↦ₐ wentry
+    ∗ ▷ (PC ↦ᵣ WCap pc_p pc_g pc_b pc_e a_last
+         ∗ rdst ↦ᵣ load_word pc_p wentry
+         ∗ rscratch1 ↦ᵣ WInt 0%Z
+         ∗ rscratch2 ↦ᵣ WInt 0%Z
+         ∗ codefrag pc_a fetch
+         ∗ (pc_b ^+ n)%a ↦ₐ wentry
+         -∗ WP Seq (Instr Executable) {{ φ }})
+    ⊢ WP Seq (Instr Executable) {{ φ }}.
   Proof.
-    iIntros (Hvpc Hcont Hwb Hentry) "(>Hprog & >HPC & >Hpc_b & >Ha_entry & >Hr_t1 & >Hr_t2 & >Hr_t3 & Hφ)".
+    intros fetch a_last ; subst fetch a_last.
+    iIntros (Hvpc Hcont Hpc_n)
+      "(>HPC & >Hrdst & >Hrscratch1 & >Hrscratch2 & >Hprog & >Hpc_bn & Hφ)".
     iDestruct (big_sepL2_length with "Hprog") as %Hlength.
-    destruct a as [|a l];[inversion Hlength|].
-    apply contiguous_between_cons_inv_first in Hcont as Heq. subst.
-    (* move r_t1 PC *)
-    destruct l;[inversion Hlength|].
-    iPrologue "Hprog".
-    iApply (wp_move_success_reg_fromPC with "[$HPC $Hi $Hr_t1]");
-      [apply decode_encode_instrW_inv|iCorrectPC a_first a_last|iContiguous_next Hcont 0|auto|..].
-    iEpilogue "(HPC & Hprog_done & Hr_t1)".
-    (* getb r_t2 r_t1 *)
-    destruct l;[inversion Hlength|].
-    iPrologue "Hprog".
-    iApply (wp_Get_success with "[$HPC $Hi $Hr_t1 $Hr_t2 ]");
-      [apply decode_encode_instrW_inv|auto|iCorrectPC a_first a_last|iContiguous_next Hcont 1|auto..].
-    iEpilogue "(HPC & Hi & Hr_t1 & Hr_t2) /="; iCombine "Hi" "Hprog_done" as "Hprog_done".
-    (* geta r_t3 r_t1 *)
-    destruct l;[inversion Hlength|].
-    iPrologue "Hprog".
-    iApply (wp_Get_success with "[$HPC $Hi $Hr_t1 $Hr_t3]");
-      [apply decode_encode_instrW_inv|auto|iCorrectPC a_first a_last|iContiguous_next Hcont 2|auto..].
-    iEpilogue "(HPC & Hi & Hr_t1 & Hr_t3) /="; iCombine "Hi" "Hprog_done" as "Hprog_done".
-    (* sub r_t2 r_t2 r_t3 *)
-    destruct l;[inversion Hlength|].
-    iPrologue "Hprog".
-    iApply (wp_binop_success_dst_r with "[$HPC $Hi $Hr_t3 $Hr_t2]");
-      [apply decode_encode_instrW_inv|auto|iContiguous_next Hcont 3|iCorrectPC a_first a_last|..].
-    iEpilogue "(HPC & Hi & Hr_t3 & Hr_t2) /="; iCombine "Hi" "Hprog_done" as "Hprog_done".
-    (* lea r_t1 r_t2 *)
-    destruct l;[inversion Hlength|].
-    iPrologue "Hprog".
-    assert ((a_first + (pc_b - a_first))%a = Some pc_b) as Hlea;[solve_addr|].
-    iApply (wp_lea_success_reg with "[$HPC $Hi $Hr_t1 $Hr_t2]");
-      [apply decode_encode_instrW_inv|iCorrectPC a_first a_last|iContiguous_next Hcont 4|apply Hlea|auto..].
-    { apply contiguous_between_length in Hcont.
-      apply isCorrectPC_range_perm in Hvpc; [|revert Hcont; clear; solve_addr].
-      destruct Hvpc as [-> | ->]; auto. }
-    iEpilogue "(HPC & Hi & Hr_t2 & Hr_t1) /="; iCombine "Hi" "Hprog_done" as "Hprog_done".
-    (* load r_t1 r_t1 *)
-    destruct l;[inversion Hlength|].
-    iPrologue "Hprog".
-    iAssert (⌜(pc_b ≠ f4)%Z⌝)%I as %Hneq.
-    { iIntros (Hcontr);subst. iApply (addr_dupl_false with "Hi Hpc_b"). }
-    iApply (wp_load_success_same with "[$HPC $Hi $Hr_t1 Hpc_b]");
-      [|apply decode_encode_instrW_inv|iCorrectPC a_first a_last| | |iContiguous_next Hcont 5|..].
-    { exact (WCap RW b_link e_link a_link). }
-    { apply contiguous_between_length in Hcont as Hlen.
-      assert (pc_b < pc_e)%Z as Hle.
-      { eapply isCorrectPC_contiguous_range in Hvpc as Hwb';[|eauto|apply elem_of_cons;left;eauto].
-        inversion Hwb'. solve_addr. }
-      apply isCorrectPC_range_perm in Hvpc as Heq; [|revert Hlen; clear; solve_addr].
-      destruct Heq as [-> | ->]; auto. }
-    { apply andb_true_intro. split;[apply Z.leb_le;solve_addr|apply Z.ltb_lt;auto].
-      assert (pc_b < pc_e)%Z as Hle.
-      { eapply isCorrectPC_contiguous_range in Hvpc as Hwb';[|eauto|apply elem_of_cons;left;eauto].
-        inversion Hwb'. solve_addr. } auto. }
-    { destruct (pc_b =? f4)%a; [done|iFrame]. }
-    destruct ((pc_b =? f4)%a) eqn:Hcontr;[apply Z.eqb_eq in Hcontr;apply finz_to_z_eq in Hcontr;congruence|clear Hcontr].
-    iEpilogue "(HPC & Hr_t1 & Hi & Hpc_b)"; iCombine "Hi" "Hprog_done" as "Hprog_done".
-    (* lea r_t1 f *)
-    destruct l;[inversion Hlength|].
-    iPrologue "Hprog".
-    iApply (wp_lea_success_z with "[$HPC $Hi $Hr_t1]");
-      [apply decode_encode_instrW_inv|iCorrectPC a_first a_last|iContiguous_next Hcont 6|apply Hentry|simpl;auto..].
-    iEpilogue "(HPC & Hi & Hr_t1)"; iCombine "Hi" "Hprog_done" as "Hprog_done".
-    (* move r_t2 0 *)
-    destruct l;[inversion Hlength|].
-    iPrologue "Hprog".
-    iApply (wp_move_success_z with "[$HPC $Hi $Hr_t2]");
-      [apply decode_encode_instrW_inv|iCorrectPC a_first a_last|iContiguous_next Hcont 7|auto|..].
-    iEpilogue "(HPC & Hi & Hr_t2)"; iCombine "Hi" "Hprog_done" as "Hprog_done".
-    (* move r_t3 0 *)
-    destruct l;[inversion Hlength|].
-    iPrologue "Hprog".
-    iApply (wp_move_success_z with "[$HPC $Hi $Hr_t3]");
-      [apply decode_encode_instrW_inv|iCorrectPC a_first a_last|iContiguous_next Hcont 8|auto|..].
-    iEpilogue "(HPC & Hi & Hr_t3)"; iCombine "Hi" "Hprog_done" as "Hprog_done".
-    (* load r_t1 r_t1 *)
-    destruct l;[|inversion Hlength].
-    apply contiguous_between_last with (ai:=f8) in Hcont as Hlink;[|auto].
-    iPrologue "Hprog".
-    iAssert (⌜(entry_a ≠ f8)%Z⌝)%I as %Hneq'.
-    { iIntros (Hcontr);subst. iApply (addr_dupl_false with "Hi Ha_entry"). }
-    iApply (wp_load_success_same with "[$HPC $Hi $Hr_t1 Ha_entry]");
-      [exact wentry|apply decode_encode_instrW_inv|iCorrectPC a_first a_last|auto|auto|apply Hlink|..].
-    { destruct (entry_a =? f8)%a; auto. }
-    destruct ((entry_a =? f8)%a) eqn:Hcontr;[apply Z.eqb_eq in Hcontr;apply finz_to_z_eq in Hcontr;congruence|clear Hcontr].
-    iEpilogue "(HPC & Hr_t1 & Hi & Hentry_a)"; iCombine "Hi" "Hprog_done" as "Hprog_done".
-    (* continuation *)
-    iApply "Hφ".
-    iFrame.
-    do 9 iDestruct "Hprog_done" as "[$ Hprog_done]".
-    iFrame.
+    codefrag_facts "Hprog".
+    rename H into HcontRegion; clear H0.
+    assert ((pc_a + (pc_b - pc_a))%a = Some pc_b) as Hlea;[solve_addr|].
+    assert ((pc_b + n)%a = Some (pc_b ^+ n)%a) as Hpc_bn;[solve_addr|].
+    iGo "Hprog".
+    iApply "Hφ"; iFrame.
   Qed.
 
 End Fetch.
